doc-src/TutorialI/Protocol/Event.thy
@@ -3,16 +3,15 @@
     Author:     Lawrence C Paulson, Cambridge University Computer Laboratory
     Copyright   1996  University of Cambridge
 
-Theory of events for security protocols
-
 Datatype of events; function "spies"; freshness
 
 "bad" agents have been broken by the Spy; their private keys and internal
     stores are visible to him
-*)
+*)(*<*)
 
-theory Event imports Message
-uses ("Event_lemmas.ML") begin
+header{*Theory of Events for Security Protocols*}
+
+theory Event imports Message begin
 
 consts  (*Initial states of agents -- parameter of the construction*)
   initState :: "agent => msg set"
@@ -27,18 +26,17 @@ consts
   knows  :: "agent => event list => msg set"
 
 
-(*"spies" is retained for compatibility's sake*)
-syntax
-  spies  :: "event list => msg set"
+text{*The constant "spies" is retained for compatibility's sake*}
 
-translations
-  "spies"   => "knows Spy"
+abbreviation (input)
+  spies  :: "event list => msg set" where
+  "spies == knows Spy"
 
-
-axioms
-  (*Spy has access to his own key for spoof messages, but Server is secure*)
-  Spy_in_bad     [iff] :    "Spy \<in> bad"
-  Server_not_bad [iff] : "Server \<notin> bad"
+text{*Spy has access to his own key for spoof messages, but Server is secure*}
+specification (bad)
+  Spy_in_bad     [iff]: "Spy \<in> bad"
+  Server_not_bad [iff]: "Server \<notin> bad"
+    by (rule exI [of _ "{Spy}"], simp)
 
 primrec
   knows_Nil:   "knows A [] = initState A"
@@ -74,16 +72,321 @@ primrec
   used_Nil:   "used []         = (UN B. parts (initState B))"
   used_Cons:  "used (ev # evs) =
 		     (case ev of
-			Says A B X => parts {X} Un (used evs)
+			Says A B X => parts {X} \<union> used evs
 		      | Gets A X   => used evs
-		      | Notes A X  => parts {X} Un (used evs))"
+		      | Notes A X  => parts {X} \<union> used evs)"
+    --{*The case for @{term Gets} seems anomalous, but @{term Gets} always
+        follows @{term Says} in real protocols.  Seems difficult to change.
+        See @{text Gets_correct} in theory @{text "Guard/Extensions.thy"}. *}
+
+lemma Notes_imp_used [rule_format]: "Notes A X \<in> set evs --> X \<in> used evs"
+apply (induct_tac evs)
+apply (auto split: event.split) 
+done
+
+lemma Says_imp_used [rule_format]: "Says A B X \<in> set evs --> X \<in> used evs"
+apply (induct_tac evs)
+apply (auto split: event.split) 
+done
 
 
-use "Event_lemmas.ML"
+subsection{*Function @{term knows}*}
+
+(*Simplifying   
+ parts(insert X (knows Spy evs)) = parts{X} \<union> parts(knows Spy evs).
+  This version won't loop with the simplifier.*)
+lemmas parts_insert_knows_A = parts_insert [of _ "knows A evs", standard]
+
+lemma knows_Spy_Says [simp]:
+     "knows Spy (Says A B X # evs) = insert X (knows Spy evs)"
+by simp
+
+text{*Letting the Spy see "bad" agents' notes avoids redundant case-splits
+      on whether @{term "A=Spy"} and whether @{term "A\<in>bad"}*}
+lemma knows_Spy_Notes [simp]:
+     "knows Spy (Notes A X # evs) =  
+          (if A:bad then insert X (knows Spy evs) else knows Spy evs)"
+by simp
+
+lemma knows_Spy_Gets [simp]: "knows Spy (Gets A X # evs) = knows Spy evs"
+by simp
+
+lemma knows_Spy_subset_knows_Spy_Says:
+     "knows Spy evs \<subseteq> knows Spy (Says A B X # evs)"
+by (simp add: subset_insertI)
+
+lemma knows_Spy_subset_knows_Spy_Notes:
+     "knows Spy evs \<subseteq> knows Spy (Notes A X # evs)"
+by force
+
+lemma knows_Spy_subset_knows_Spy_Gets:
+     "knows Spy evs \<subseteq> knows Spy (Gets A X # evs)"
+by (simp add: subset_insertI)
+
+text{*Spy sees what is sent on the traffic*}
+lemma Says_imp_knows_Spy [rule_format]:
+     "Says A B X \<in> set evs --> X \<in> knows Spy evs"
+apply (induct_tac "evs")
+apply (simp_all (no_asm_simp) split add: event.split)
+done
+
+lemma Notes_imp_knows_Spy [rule_format]:
+     "Notes A X \<in> set evs --> A: bad --> X \<in> knows Spy evs"
+apply (induct_tac "evs")
+apply (simp_all (no_asm_simp) split add: event.split)
+done
+
+
+text{*Elimination rules: derive contradictions from old Says events containing
+  items known to be fresh*}
+lemmas knows_Spy_partsEs =
+     Says_imp_knows_Spy [THEN parts.Inj, THEN revcut_rl, standard] 
+     parts.Body [THEN revcut_rl, standard]
+
+lemmas Says_imp_analz_Spy = Says_imp_knows_Spy [THEN analz.Inj]
+
+text{*Compatibility for the old "spies" function*}
+lemmas spies_partsEs = knows_Spy_partsEs
+lemmas Says_imp_spies = Says_imp_knows_Spy
+lemmas parts_insert_spies = parts_insert_knows_A [of _ Spy]
+
+
+subsection{*Knowledge of Agents*}
+
+lemma knows_Says: "knows A (Says A B X # evs) = insert X (knows A evs)"
+by simp
+
+lemma knows_Notes: "knows A (Notes A X # evs) = insert X (knows A evs)"
+by simp
+
+lemma knows_Gets:
+     "A \<noteq> Spy --> knows A (Gets A X # evs) = insert X (knows A evs)"
+by simp
+
+
+lemma knows_subset_knows_Says: "knows A evs \<subseteq> knows A (Says A' B X # evs)"
+by (simp add: subset_insertI)
+
+lemma knows_subset_knows_Notes: "knows A evs \<subseteq> knows A (Notes A' X # evs)"
+by (simp add: subset_insertI)
+
+lemma knows_subset_knows_Gets: "knows A evs \<subseteq> knows A (Gets A' X # evs)"
+by (simp add: subset_insertI)
+
+text{*Agents know what they say*}
+lemma Says_imp_knows [rule_format]: "Says A B X \<in> set evs --> X \<in> knows A evs"
+apply (induct_tac "evs")
+apply (simp_all (no_asm_simp) split add: event.split)
+apply blast
+done
+
+text{*Agents know what they note*}
+lemma Notes_imp_knows [rule_format]: "Notes A X \<in> set evs --> X \<in> knows A evs"
+apply (induct_tac "evs")
+apply (simp_all (no_asm_simp) split add: event.split)
+apply blast
+done
+
+text{*Agents know what they receive*}
+lemma Gets_imp_knows_agents [rule_format]:
+     "A \<noteq> Spy --> Gets A X \<in> set evs --> X \<in> knows A evs"
+apply (induct_tac "evs")
+apply (simp_all (no_asm_simp) split add: event.split)
+done
+
+
+text{*What agents DIFFERENT FROM Spy know 
+  was either said, or noted, or got, or known initially*}
+lemma knows_imp_Says_Gets_Notes_initState [rule_format]:
+     "[| X \<in> knows A evs; A \<noteq> Spy |] ==> EX B.  
+  Says A B X \<in> set evs | Gets A X \<in> set evs | Notes A X \<in> set evs | X \<in> initState A"
+apply (erule rev_mp)
+apply (induct_tac "evs")
+apply (simp_all (no_asm_simp) split add: event.split)
+apply blast
+done
+
+text{*What the Spy knows -- for the time being --
+  was either said or noted, or known initially*}
+lemma knows_Spy_imp_Says_Notes_initState [rule_format]:
+     "[| X \<in> knows Spy evs |] ==> EX A B.  
+  Says A B X \<in> set evs | Notes A X \<in> set evs | X \<in> initState Spy"
+apply (erule rev_mp)
+apply (induct_tac "evs")
+apply (simp_all (no_asm_simp) split add: event.split)
+apply blast
+done
+
+lemma parts_knows_Spy_subset_used: "parts (knows Spy evs) \<subseteq> used evs"
+apply (induct_tac "evs", force)  
+apply (simp add: parts_insert_knows_A knows_Cons add: event.split, blast) 
+done
+
+lemmas usedI = parts_knows_Spy_subset_used [THEN subsetD, intro]
+
+lemma initState_into_used: "X \<in> parts (initState B) ==> X \<in> used evs"
+apply (induct_tac "evs")
+apply (simp_all add: parts_insert_knows_A split add: event.split, blast)
+done
+
+lemma used_Says [simp]: "used (Says A B X # evs) = parts{X} \<union> used evs"
+by simp
+
+lemma used_Notes [simp]: "used (Notes A X # evs) = parts{X} \<union> used evs"
+by simp
+
+lemma used_Gets [simp]: "used (Gets A X # evs) = used evs"
+by simp
+
+lemma used_nil_subset: "used [] \<subseteq> used evs"
+apply simp
+apply (blast intro: initState_into_used)
+done
+
+text{*NOTE REMOVAL--laws above are cleaner, as they don't involve "case"*}
+declare knows_Cons [simp del]
+        used_Nil [simp del] used_Cons [simp del]
+
+
+text{*For proving theorems of the form @{term "X \<notin> analz (knows Spy evs) --> P"}
+  New events added by induction to "evs" are discarded.  Provided 
+  this information isn't needed, the proof will be much shorter, since
+  it will omit complicated reasoning about @{term analz}.*}
+
+lemmas analz_mono_contra =
+       knows_Spy_subset_knows_Spy_Says [THEN analz_mono, THEN contra_subsetD]
+       knows_Spy_subset_knows_Spy_Notes [THEN analz_mono, THEN contra_subsetD]
+       knows_Spy_subset_knows_Spy_Gets [THEN analz_mono, THEN contra_subsetD]
+
+ML
+{*
+val analz_mono_contra_tac = 
+  let val analz_impI = inst "P" "?Y \<notin> analz (knows Spy ?evs)" impI
+  in
+    rtac analz_impI THEN' 
+    REPEAT1 o 
+      (dresolve_tac (thms"analz_mono_contra"))
+    THEN' mp_tac
+  end
+*}
+
+
+lemma knows_subset_knows_Cons: "knows A evs \<subseteq> knows A (e # evs)"
+by (induct e, auto simp: knows_Cons)
+
+lemma initState_subset_knows: "initState A \<subseteq> knows A evs"
+apply (induct_tac evs, simp) 
+apply (blast intro: knows_subset_knows_Cons [THEN subsetD])
+done
+
+
+text{*For proving @{text new_keys_not_used}*}
+lemma keysFor_parts_insert:
+     "[| K \<in> keysFor (parts (insert X G));  X \<in> synth (analz H) |] 
+      ==> K \<in> keysFor (parts (G \<union> H)) | Key (invKey K) \<in> parts H"; 
+by (force 
+    dest!: parts_insert_subset_Un [THEN keysFor_mono, THEN [2] rev_subsetD]
+           analz_subset_parts [THEN keysFor_mono, THEN [2] rev_subsetD]
+    intro: analz_subset_parts [THEN subsetD] parts_mono [THEN [2] rev_subsetD])
 
 method_setup analz_mono_contra = {*
-    Method.no_args
-      (Method.METHOD (fn facts => REPEAT_FIRST analz_mono_contra_tac)) *}
+    Method.no_args (Method.SIMPLE_METHOD (REPEAT_FIRST analz_mono_contra_tac)) *}
     "for proving theorems of the form X \<notin> analz (knows Spy evs) --> P"
 
+subsubsection{*Useful for case analysis on whether a hash is a spoof or not*}
+
+ML
+{*
+val knows_Cons     = thm "knows_Cons"
+val used_Nil       = thm "used_Nil"
+val used_Cons      = thm "used_Cons"
+
+val Notes_imp_used = thm "Notes_imp_used";
+val Says_imp_used = thm "Says_imp_used";
+val Says_imp_knows_Spy = thm "Says_imp_knows_Spy";
+val Notes_imp_knows_Spy = thm "Notes_imp_knows_Spy";
+val knows_Spy_partsEs = thms "knows_Spy_partsEs";
+val spies_partsEs = thms "spies_partsEs";
+val Says_imp_spies = thm "Says_imp_spies";
+val parts_insert_spies = thm "parts_insert_spies";
+val Says_imp_knows = thm "Says_imp_knows";
+val Notes_imp_knows = thm "Notes_imp_knows";
+val Gets_imp_knows_agents = thm "Gets_imp_knows_agents";
+val knows_imp_Says_Gets_Notes_initState = thm "knows_imp_Says_Gets_Notes_initState";
+val knows_Spy_imp_Says_Notes_initState = thm "knows_Spy_imp_Says_Notes_initState";
+val usedI = thm "usedI";
+val initState_into_used = thm "initState_into_used";
+val used_Says = thm "used_Says";
+val used_Notes = thm "used_Notes";
+val used_Gets = thm "used_Gets";
+val used_nil_subset = thm "used_nil_subset";
+val analz_mono_contra = thms "analz_mono_contra";
+val knows_subset_knows_Cons = thm "knows_subset_knows_Cons";
+val initState_subset_knows = thm "initState_subset_knows";
+val keysFor_parts_insert = thm "keysFor_parts_insert";
+
+
+val synth_analz_mono = thm "synth_analz_mono";
+
+val knows_Spy_subset_knows_Spy_Says = thm "knows_Spy_subset_knows_Spy_Says";
+val knows_Spy_subset_knows_Spy_Notes = thm "knows_Spy_subset_knows_Spy_Notes";
+val knows_Spy_subset_knows_Spy_Gets = thm "knows_Spy_subset_knows_Spy_Gets";
+
+
+val synth_analz_mono_contra_tac = 
+  let val syan_impI = inst "P" "?Y \<notin> synth (analz (knows Spy ?evs))" impI
+  in
+    rtac syan_impI THEN' 
+    REPEAT1 o 
+      (dresolve_tac 
+       [knows_Spy_subset_knows_Spy_Says RS synth_analz_mono RS contra_subsetD,
+        knows_Spy_subset_knows_Spy_Notes RS synth_analz_mono RS contra_subsetD,
+	knows_Spy_subset_knows_Spy_Gets RS synth_analz_mono RS contra_subsetD])
+    THEN'
+    mp_tac
+  end;
+*}
+
+method_setup synth_analz_mono_contra = {*
+    Method.no_args (Method.SIMPLE_METHOD (REPEAT_FIRST synth_analz_mono_contra_tac)) *}
+    "for proving theorems of the form X \<notin> synth (analz (knows Spy evs)) --> P"
+(*>*)
+
+section{* Event Traces \label{sec:events} *}
+
+text {*
+The system's behaviour is formalized as a set of traces of
+\emph{events}.  The most important event, @{text "Says A B X"}, expresses
+$A\to B : X$, which is the attempt by~$A$ to send~$B$ the message~$X$.
+A trace is simply a list, constructed in reverse
+using~@{text "#"}.  Other event types include reception of messages (when
+we want to make it explicit) and an agent's storing a fact.
+
+Sometimes the protocol requires an agent to generate a new nonce. The
+probability that a 20-byte random number has appeared before is effectively
+zero.  To formalize this important property, the set @{term "used evs"}
+denotes the set of all items mentioned in the trace~@{text evs}.
+The function @{text used} has a straightforward
+recursive definition.  Here is the case for @{text Says} event:
+@{thm [display,indent=5] used_Says [no_vars]}
+
+The function @{text knows} formalizes an agent's knowledge.  Mostly we only
+care about the spy's knowledge, and @{term "knows Spy evs"} is the set of items
+available to the spy in the trace~@{text evs}.  Already in the empty trace,
+the spy starts with some secrets at his disposal, such as the private keys
+of compromised users.  After each @{text Says} event, the spy learns the
+message that was sent:
+@{thm [display,indent=5] knows_Spy_Says [no_vars]}
+Combinations of functions express other important
+sets of messages derived from~@{text evs}:
+\begin{itemize}
+\item @{term "analz (knows Spy evs)"} is everything that the spy could
+learn by decryption
+\item @{term "synth (analz (knows Spy evs))"} is everything that the spy
+could generate
+\end{itemize}
+*}
+
+(*<*)
 end
+(*>*)
